README.md
@@ -1,8 +1,13 @@
 # Lean Substitution Library (lean-subst)
 
-Inspired heavily by the work on Autosubst [[1]](https://doi.org/10.1007/978-3-319-22102-1_24) [[2]](https://dl.acm.org/doi/10.1145/3293880.3294101), this library gives a framework for handling De Bruijn substitution for non-indexed single-sorted syntax. Other Autosubst inspired systems supported multi-sorted syntax by way of multi-sorted substitutions (i.e., `t[σ;τ]` substitutes for the term and type variables via two separate substitutions). This library instead allows variables to be annotated with extra data. For example, `var : VarKind -> Nat -> Term` where `VarKind = Term | Type` encodes the multi-sorted idea using only variable constructor and hence one substitution.
+Inspired heavily by the work on Autosubst [[1]](https://doi.org/10.1007/978-3-319-22102-1_24) [[2]](https://dl.acm.org/doi/10.1145/3293880.3294101), this library gives a framework for handling De Bruijn substitution for non-indexed syntax.
 
-This accomplished by treating substitutions as sequences of "substitution actions":
+Features:
+1. Heterogenous simultaneous substitutions (like the original Autosubst in Rocq)
+2. Variables can track additional data (because renamings embed into substitutions)
+3. Annotations for `simp` and `grind` enabling automation of the convergent rewriting system described in the Autosubst literature
+
+Variables tracking additional data is accomplished by treating substitutions as sequences of "substitution actions":
 ```lean
 inductive Action T where
 | su : T -> Action T
@@ -12,9 +17,10 @@ Subst T := Nat -> Action T
 ```
 The `su` constructor encodes a genuine replacement for a variable at the right index with a term. The `re` constructor encodes a renaming where a variable constructor's annotated data is preserved and only its index is modified.
 
-This library supports only mediocre macro support. A user must provide a definition of `smap` that properly handles variables and binders. Additionally, one must prove a host of simplification lemmas that communicate how substitutions commute through the structure of a term. Finally, the required type classes `SubstStable` and `SubstCompose` must be defined, but useful tactics are provided to prove these goals automatically.
-
-Because facts about reduction are usually tightly tied ones handling of substitution this library also includes some basic theory of abstract rewriting in `LeanSubst/Reduction.lean` and `LeanSubst/Normal.lean`.
+TODO:
+1. Generalization to vector substitutions
+2. Support for well-scoped De Bruijn
+1. Automatic derivation of substitution definitions, lemmas and typeclasses
 
 # Usage
 
@@ -30,7 +36,8 @@ rev = "main"
 
 Change `rev` to a release tag or pinned commit as desired, then run `lake update`.
 
-Syntax must be non-indexed and single-sorted, see "Examples" for the various requirements needed to properly set up an inductive type encoding syntax.
+Syntax must be non-indexed, see "Examples" for the various requirements needed to properly set up an inductive type encoding syntax.
 
 Other non-trivial uses of this library are available here:
-1. [A formalization of the metatheory of STLC](https://github.com/amarmaduke/lean-stlc)
+1. [A mechanization of the metatheory of STLC](https://github.com/amarmaduke/lean-stlc)
+2. [A mechanization of the metatheory of System F](https://github.com/amarmaduke/lean-sysf)
